Proof of add_alloc for the finite language.
Some cleanup of nested lemmas.

src/coq/Theory/OOMRefinementExamples.v
@@ -28,6 +28,52 @@ Import DynamicTypes.
 Require Import Morphisms.
 Require Import Paco.paco.
 
+
+(* TODO: Move all of this stuff *)
+Lemma ret_map_itree :
+  forall Eff A B (f : A -> B) (t : itree Eff A) (a : A),
+    ITree.map f t ≈ ret (f a) ->
+    exists a', t ≈ ret a' /\ f a' = f a.
+Proof.
+Admitted.
+
+Lemma itree_map_ret_inv :
+  forall {E X Y} f (t : itree E X) (y : Y),
+    ITree.map f t ≈ ret y ->
+    exists (x : X), t ≈ ret x /\ f x = y.
+Proof.
+Admitted.
+
+Class KSPEC_WF {E F} (h_spec : forall T : Type, E T -> PropT F T)
+      (k_spec : forall T R : Type, E T -> itree F T -> (T -> itree F R) -> itree F R -> Prop) : Type
+  := k_spec_WF_class : k_spec_WF h_spec k_spec.
+
+#[global] Instance interp_prop_eutt_Proper2:
+  forall {E F : Type -> Type} {h_spec : forall T : Type, E T -> PropT F T}
+    {k_spec : forall T R : Type, E T -> itree F T -> (T -> itree F R) -> itree F R -> Prop}
+    `{WF : @KSPEC_WF _ _ h_spec k_spec},
+  forall (R : Type) (RR : Relation_Definitions.relation R),
+    Proper (eutt eq ==> eutt eq ==> iff) (interp_prop h_spec k_spec R RR).
+Proof.
+  intros E F h_spec k_spec H R RR.
+  unfold Proper, respectful.
+  intros x y H0 x0 y0 H1.
+  split; intros H2.
+  - eapply interp_prop_eutt_Proper; eauto.
+    symmetry; auto.
+    symmetry; auto.
+  - eapply interp_prop_eutt_Proper; eauto.
+Qed.
+
+Lemma interp_prop_vis :
+  forall {E F X} (h_spec : E ~> PropT F) k_spec R RR
+    (e : E X) kk t,
+    interp_prop h_spec k_spec R RR (Vis e kk) t <->
+      (x <- h_spec X e;;
+       interp_prop h_spec k_spec R RR (kk x)) t. (* Do I need to use k_spec anywhere...? *)
+Proof.
+Admitted.
+
 Module Infinite.
   Import TopLevelBigIntptr.
   Import TopLevelRefinementsBigIntptr.
@@ -59,6 +105,63 @@ Module Infinite.
   Import ListNotations.
   Require Import Coq.Strings.String.
 
+  (* TODO: Move these *)
+  #[global] Instance KSPEC_poison :
+    KSPEC_WF
+      (case_ (E_trigger_prop (F:=OOME +' UBE +' DebugE +' FailureE))
+             (case_ PickUvalue_handler (F_trigger_prop (F:=OOME +' UBE +' DebugE +' FailureE))))
+      (@pick_uvalue_k_spec ExternalCallE (OOME +' UBE +' DebugE +' FailureE)).
+  Proof.
+    apply k_spec_WF_pick_uvalue_k_spec.
+  Defined.
+
+  #[global] Instance KSPEC_memory {sid m} :
+    KSPEC_WF
+      (fun (T : Type)
+         (e : (ExternalCallE +'
+                                LLVMParamsBigIntptr.Events.IntrinsicE +'
+                                                                         LLVMParamsBigIntptr.Events.MemoryE +' PickUvalueE +' OOME +' UBE +' DebugE +' FailureE) T)
+         (t : itree (ExternalCallE +' PickUvalueE +' OOME +' UBE +' DebugE +' FailureE) T) =>
+         exists (sid' : store_id) (ms' : MMEP.MMSP.MemState),
+           interp_memory_prop_h e sid m (ITree.map (fun x : T => (ms', (sid', x))) t))
+      (@memory_k_spec ExternalCallE (PickUvalueE +' OOME +' UBE +' DebugE +' FailureE)).
+  Proof.
+    apply k_spec_WF_memory_k_spec.
+  Defined.
+
+  #[global] Instance interp_mem_prop_Proper3 :
+    forall {E F} `{FAIL : FailureE -< F} `{UB : UBE -< F} `{OOM : OOME -< F}
+      {R} (RR : R -> R -> Prop),
+      Proper (eutt eq ==> eq ==> eq ==> eq ==> iff) (@interp_memory_prop E F FAIL UB OOM R RR).
+  Proof.
+    intros E F FAIL UB OOM R RR.
+    unfold interp_memory_prop.
+    unfold Proper, respectful.
+    intros x y H x0 y0 H0 x1 y1 H1 x2 y2 H2.
+    subst.
+    split; intros INTERP.
+    - eapply interp_prop_eutt_Proper_impl.
+      + admit.
+      + eauto.
+      + reflexivity.
+      + auto.
+    - eapply interp_prop_eutt_Proper_impl.
+      + admit.
+      + symmetry. apply H.
+      + reflexivity.
+      + auto.
+  Admitted.
+
+  (* TODO: Move this *)
+  Import Relation_Definitions.
+  #[global] Instance refine_OOM_h_eutt_Proper {T : Type} {RR : relation T} {E F}:
+    Proper (eutt eq ==> eutt eq ==> iff) (@refine_OOM_h E F T RR).
+  Proof.
+    unfold Proper, respectful.
+    intros x1 x2 X y1 y2 Y.
+    split; intros REFINE.
+  Admitted.
+  
   Definition alloc_code : code dtyp :=
     [ (IId (Name "ptr"), INSTR_Alloca (DTYPE_I 64%N) None None)
     ].
@@ -146,33 +249,6 @@ Module Infinite.
 
       destruct INTERP as [t_pre [INTERP UNDEF]].
 
-      (* TODO: Need something about interp_memory_prop being proper with respect to eutt? *)
-      (* Not sure if this is exactly what it should be *)
-
-      Set Nested Proofs Allowed.
-      #[global] Instance interp_mem_prop_Proper3 :
-        forall {E F} `{FAIL : FailureE -< F} `{UB : UBE -< F} `{OOM : OOME -< F}
-          {R} (RR : R -> R -> Prop),
-          Proper (eutt eq ==> eq ==> eq ==> eq ==> iff) (@interp_memory_prop E F FAIL UB OOM R RR).
-      Proof.
-        intros E F FAIL UB OOM R RR.
-        unfold interp_memory_prop.
-        unfold Proper, respectful.
-        intros x y H x0 y0 H0 x1 y1 H1 x2 y2 H2.
-        subst.
-        split; intros INTERP.
-        - eapply interp_prop_eutt_Proper_impl.
-          + admit.
-          + eauto.
-          + reflexivity.
-          + auto.
-        - eapply interp_prop_eutt_Proper_impl.
-          + admit.
-          + symmetry. apply H.
-          + reflexivity.
-          + auto.
-      Admitted.
-
       setoid_rewrite interp_intrinsics_ret in INTERP.
       setoid_rewrite interp_global_ret in INTERP.
       setoid_rewrite interp_local_stack_ret in INTERP.
@@ -188,57 +264,6 @@ Module Infinite.
       auto.
       clear EQ.
       rename H into EQ.
-
-      Lemma ret_map_itree :
-        forall Eff A B (f : A -> B) (t : itree Eff A) (a : A),
-          ITree.map f t ≈ ret (f a) ->
-          exists a', t ≈ ret a' /\ f a' = f a.
-      Proof.
-      Admitted.
-
-      Class KSPEC_WF {E F} (h_spec : forall T : Type, E T -> PropT F T)
-            (k_spec : forall T R : Type, E T -> itree F T -> (T -> itree F R) -> itree F R -> Prop) : Type
-        := k_spec_WF_class : k_spec_WF h_spec k_spec.
-
-      #[global] Instance interp_prop_eutt_Proper2:
-        forall {E F : Type -> Type} {h_spec : forall T : Type, E T -> PropT F T}
-          {k_spec : forall T R : Type, E T -> itree F T -> (T -> itree F R) -> itree F R -> Prop}
-          `{WF : @KSPEC_WF _ _ h_spec k_spec},
-          forall (R : Type) (RR : Relation_Definitions.relation R),
-            Proper (eutt eq ==> eutt eq ==> iff) (interp_prop h_spec k_spec R RR).
-      Proof.
-        intros E F h_spec k_spec H R RR.
-        unfold Proper, respectful.
-        intros x y H0 x0 y0 H1.
-        split; intros H2.
-        - eapply interp_prop_eutt_Proper; eauto.
-          symmetry; auto.
-          symmetry; auto.
-        - eapply interp_prop_eutt_Proper; eauto.
-      Qed.
-
-      #[global] Instance KSPEC_poison :
-        KSPEC_WF
-          (case_ (E_trigger_prop (F:=OOME +' UBE +' DebugE +' FailureE))
-                 (case_ PickUvalue_handler (F_trigger_prop (F:=OOME +' UBE +' DebugE +' FailureE))))
-          (@pick_uvalue_k_spec ExternalCallE (OOME +' UBE +' DebugE +' FailureE)).
-      Proof.
-        apply k_spec_WF_pick_uvalue_k_spec.
-      Defined.
-
-      #[global] Instance KSPEC_memory {sid m} :
-        KSPEC_WF
-          (fun (T : Type)
-             (e : (ExternalCallE +'
-                                    LLVMParamsBigIntptr.Events.IntrinsicE +'
-                                                                             LLVMParamsBigIntptr.Events.MemoryE +' PickUvalueE +' OOME +' UBE +' DebugE +' FailureE) T)
-             (t : itree (ExternalCallE +' PickUvalueE +' OOME +' UBE +' DebugE +' FailureE) T) =>
-             exists (sid' : store_id) (ms' : MMEP.MMSP.MemState),
-               interp_memory_prop_h e sid m (ITree.map (fun x : T => (ms', (sid', x))) t))
-          (@memory_k_spec ExternalCallE (PickUvalueE +' OOME +' UBE +' DebugE +' FailureE)).
-      Proof.
-        apply k_spec_WF_memory_k_spec.
-      Defined.
 
       apply ret_map_itree in EQ as ((m', (s', a')) & EQ & FEQ).
 
@@ -266,15 +291,6 @@ Module Infinite.
         cbn.
 
         Opaque MMEP.MemSpec.allocate_dtyp_spec.
-
-        Lemma interp_prop_vis :
-          forall {E F X} (h_spec : E ~> PropT F) k_spec R RR
-            (e : E X) kk t,
-            interp_prop h_spec k_spec R RR (Vis e kk) t <->
-            (x <- h_spec X e;;
-            interp_prop h_spec k_spec R RR (kk x)) t. (* Do I need to use k_spec anywhere...? *)
-        Proof.
-        Admitted.
 
         eapply interp_prop_vis.
         cbn.
@@ -735,17 +751,7 @@ Module Infinite.
            eapply interp_prop_ret_refine; reflexivity.
          * red.
            eapply interp_prop_ret_pure; eauto.
-      + (* TODO: Move this *)
-        Import Relation_Definitions.
-        #[global] Instance refine_OOM_h_eutt_Proper {T : Type} {RR : relation T} {E F}:
-          Proper (eutt eq ==> eutt eq ==> iff) (@refine_OOM_h E F T RR).
-        Proof.
-          unfold Proper, respectful.
-          intros x1 x2 X y1 y2 Y.
-          split; intros REFINE.
-        Admitted.
-
-        rewrite T'.
+      + rewrite T'.
         eapply refine_oom_h_raise_oom; typeclasses eauto.
     - (* Success *)
       exists (Ret5 genv (lenv, stack) sid m (DVALUE_I1 DynamicValues.Int1.one)).
@@ -767,13 +773,6 @@ Module Infinite.
         destruct ALLOC_SUC as [sid'' [ ms'' [x [MAP ALLOC_SUC]]]].        
         destruct ALLOC_SUC as [ms''' [a [ALLOC [MEQ XEQ]]]].
         subst.
-
-        Lemma itree_map_ret_inv :
-          forall {E X Y} f (t : itree E X) (y : Y),
-            ITree.map f t ≈ ret y ->
-            exists (x : X), t ≈ ret x /\ f x = y.
-        Proof.
-        Admitted.
 
         apply itree_map_ret_inv in MAP as [x [TA EQ]].
         rewrite TA in K.
@@ -822,6 +821,7 @@ Module Finite.
   Import MCFGTheory64BitIntptr.
   Import D.
 
+
   Import Global.
   Import Local.
   Import Stack.
@@ -829,208 +829,345 @@ Module Finite.
   Import MCFGTactics.
 
   Import Global.
-  Import ESID.
+  Import InterpretationStack.
+  Import InterpreterStack64BitIntptr.
+  Import MEM.
+  Import MEM_SPEC_INTERP.
 
-  Definition t_alloc : itree L0 uvalue
-    := trigger (Alloca (DTYPE_I 64%N));; ret UVALUE_None.
+  Import SemNotations.
+  Import InterpFacts.
+  Import LLVMEvents.
+  Import LLVMAst.
+  Import CFG.
 
-  Definition t_ret : itree L0 uvalue
-    := ret UVALUE_None.
+  Import List.
+  Import ListNotations.
+  Require Import Coq.Strings.String.
 
-  (* Add allocation in finite language *)
-  Lemma add_alloc :
-    forall g l s m,
-      refine_L6 (interp_mcfg4 refine_res3 t_ret g (l, s) m) (interp_mcfg4 refine_res3 t_alloc g (l, s) m).
+  Module MemTheory  := MemoryModelTheory LP MP MMEP MEM_MODEL.
+  Import MemTheory.
+
+  (* TODO: Move these *)
+  #[global] Instance KSPEC_poison :
+    KSPEC_WF
+      (case_ (E_trigger_prop (F:=OOME +' UBE +' DebugE +' FailureE))
+             (case_ PickUvalue_handler (F_trigger_prop (F:=OOME +' UBE +' DebugE +' FailureE))))
+      (@pick_uvalue_k_spec ExternalCallE (OOME +' UBE +' DebugE +' FailureE)).
   Proof.
-    intros g l s m.
+    apply k_spec_WF_pick_uvalue_k_spec.
+  Defined.
+
+  #[global] Instance KSPEC_memory {sid m} :
+    KSPEC_WF
+      (fun (T : Type)
+         (e : (ExternalCallE +'
+                                LLVMParams64BitIntptr.Events.IntrinsicE +'
+                                                                         LLVMParams64BitIntptr.Events.MemoryE +' PickUvalueE +' OOME +' UBE +' DebugE +' FailureE) T)
+         (t : itree (ExternalCallE +' PickUvalueE +' OOME +' UBE +' DebugE +' FailureE) T) =>
+         exists (sid' : store_id) (ms' : MMEP.MMSP.MemState),
+           interp_memory_prop_h e sid m (ITree.map (fun x : T => (ms', (sid', x))) t))
+      (@memory_k_spec ExternalCallE (PickUvalueE +' OOME +' UBE +' DebugE +' FailureE)).
+  Proof.
+    apply k_spec_WF_memory_k_spec.
+  Defined.
+
+  #[global] Instance interp_mem_prop_Proper3 :
+    forall {E F} `{FAIL : FailureE -< F} `{UB : UBE -< F} `{OOM : OOME -< F}
+      {R} (RR : R -> R -> Prop),
+      Proper (eutt eq ==> eq ==> eq ==> eq ==> iff) (@interp_memory_prop E F FAIL UB OOM R RR).
+  Proof.
+    intros E F FAIL UB OOM R RR.
+    unfold interp_memory_prop.
+    unfold Proper, respectful.
+    intros x y H x0 y0 H0 x1 y1 H1 x2 y2 H2.
+    subst.
+    split; intros INTERP.
+    - eapply interp_prop_eutt_Proper_impl.
+      + admit.
+      + eauto.
+      + reflexivity.
+      + auto.
+    - eapply interp_prop_eutt_Proper_impl.
+      + admit.
+      + symmetry. apply H.
+      + reflexivity.
+      + auto.
+  Admitted.
+
+  (* TODO: Move this *)
+  Import Relation_Definitions.
+  #[global] Instance refine_OOM_h_eutt_Proper {T : Type} {RR : relation T} {E F}:
+    Proper (eutt eq ==> eutt eq ==> iff) (@refine_OOM_h E F T RR).
+  Proof.
+    unfold Proper, respectful.
+    intros x1 x2 X y1 y2 Y.
+    split; intros REFINE.
+  Admitted.
+
+  (* TODO: Move this, there are duplicates of this elsewhere too. *)
+  Import TranslateFacts.
+  Ltac go_prime :=
+    repeat match goal with
+           | |- context [interp_intrinsics (ITree.bind _ _)] => rewrite interp_intrinsics_bind
+           | |- context [interp_global (ITree.bind _ _)] => rewrite interp_global_bind
+           | |- context [interp_local_stack (ITree.bind _ _)] => rewrite interp_local_stack_bind
+           (* | |- context [interp_memory (ITree.bind _ _)] => rewrite interp_memory_bind *)
+           | |- context [interp_intrinsics (trigger _)] => rewrite interp_intrinsics_trigger; cbn; rewrite ?subevent_subevent
+           | |- context [interp_intrinsics (ITree.trigger _)] => rewrite interp_intrinsics_trigger; cbn; rewrite ?subevent_subevent
+           | |- context [interp_global (trigger _)] => rewrite interp_global_trigger; cbn; rewrite ?subevent_subevent
+           | |- context [interp_global (ITree.trigger _)] => rewrite interp_global_trigger; cbn; rewrite ?subevent_subevent
+           | |- context [interp_local_stack (trigger _)] => rewrite interp_local_stack_trigger; cbn; rewrite ?subevent_subevent
+           | |- context [interp_local_stack (ITree.trigger _)] => rewrite interp_local_stack_trigger; cbn; rewrite ?subevent_subevent
+           | |- context [ITree.bind (ITree.bind _ _) _] => rewrite bind_bind
+           | |- context [interp_intrinsics (Ret _)] => rewrite interp_intrinsics_ret
+           | |- context [interp_global (Ret _)] => rewrite interp_global_ret
+           | |- context [interp_local_stack (Ret _)] => rewrite interp_local_stack_ret
+           (* | |- context [interp_memory (Ret _)] => rewrite interp_memory_ret *)
+           | |- context [ITree.bind (Ret _) _] => rewrite bind_ret_l
+           | |- context [translate _ (Ret _)] => rewrite translate_ret
+           | |- context [interp _ (trigger _)] => rewrite interp_trigger
+           | |- context [interp _ (ITree.bind _ _)] => rewrite interp_bind
+           | |- context [interp _ (Ret _)] => rewrite interp_ret
+           | |- context [map _ (ret _)] => rewrite map_ret
+           | |- context [ITree.map _ (Ret _)] => rewrite map_ret
+           | |- context [translate _ (trigger _)] => rewrite translate_trigger; cbn; rewrite ?subevent_subevent
+           | |- context [translate _ (ITree.trigger _)] => rewrite translate_trigger; cbn; rewrite ?subevent_subevent
+           | |- context [translate _ (ITree.bind _ _)] => rewrite translate_bind
+           end.
+
+  Definition alloc_code : code dtyp :=
+    [ (IId (Name "ptr"), INSTR_Alloca (DTYPE_I 64%N) None None)
+    ].
+
+  Definition ptoi_code : code dtyp :=
+    [ (IId (Name "ptr"), INSTR_Alloca (DTYPE_I 64%N) None None);
+      (IId (Name "i"), INSTR_Op (OP_Conversion Ptrtoint DTYPE_Pointer (EXP_Ident (ID_Local (Name "ptr"))) (DTYPE_IPTR)))
+    ].
+
+  Definition ret_code : code dtyp :=
+    [].
+
+  Definition alloc_block : block dtyp :=
+    {|
+      blk_id := Name "";
+      blk_phis := [];
+      blk_code := alloc_code;
+      blk_term := TERM_Ret (DTYPE_I 1%N, EXP_Bool true);
+      blk_comments := None;
+    |}.
+
+  Definition ptoi_block : block dtyp :=
+    {|
+      blk_id := Name "";
+      blk_phis := [];
+      blk_code := ptoi_code;
+      blk_term := TERM_Ret (DTYPE_I 1%N, EXP_Bool true);
+      blk_comments := None;
+    |}.
+
+  Definition ret_block : block dtyp :=
+    {|
+      blk_id := Name "";
+      blk_phis := [];
+      blk_code := ret_code;
+      blk_term := TERM_Ret (DTYPE_I 1%N, EXP_Bool true);
+      blk_comments := None;
+    |}.
+
+  Definition block_to_dvalue {E} `{FailureE -< E}
+             (t : itree E (block_id + uvalue)) : itree E dvalue :=
+    b_or_v <- t;;
+    match b_or_v with
+    | inl _ => raise "id"
+    | inr uv =>
+        match uvalue_to_dvalue uv with
+        | inl msg => raise msg
+        | inr dv => ret dv
+        end
+    end.
+
+  Definition denote_program prog :=
+    block_to_dvalue (denote_block prog (Name "blk")).
+
+  Definition alloc_tree : itree instr_E dvalue :=
+    denote_program alloc_block.
+
+  Definition ptoi_tree : itree instr_E dvalue :=
+    denote_program ptoi_block.
+
+  Definition ret_tree : itree instr_E dvalue :=
+    denote_program ret_block.
+
+  Definition t_alloc : itree L0 dvalue
+    := trigger (Alloca (DTYPE_I 64%N));; ret (DVALUE_I1 one).
+
+  Definition t_ret : itree L0 dvalue
+    := ret (DVALUE_I1 one).
+
+  (* Add allocation in the finite language *)
+  Lemma add_alloc :
+    forall genv lenv stack sid m,
+      refine_L6 (interp_mcfg4 eq eq t_ret genv (lenv, stack) sid m) (interp_mcfg4 eq eq t_alloc genv (lenv, stack) sid m).
+  Proof.
+    intros genv lenv stack sid m.
     unfold refine_L6.
     intros t' INTERP.
-    Require Import String.
-    
-    cbn in INTERP.
-    unfold interp_mcfg4 in INTERP.
 
-    unfold model_undef in INTERP.
-    go_in INTERP.
-
-    rewrite interp_memory_trigger in INTERP.
-    cbn in INTERP.
-    go_in INTERP.
-    cbn in INTERP.
-
-    (* I basically need to show that t' is the same as t_alloc, but
-       with a different effects signature..
-
-       I.e., it either OOMs or it returns UVALUE_None
+    (* either t' succeeds and we're eqv some ret like t_ret...
+       or t' runs out of memory because it's an allocation.
      *)
-    pose proof (@allocate_succeeds_or_OOMs (ms_memory_stack m) (DTYPE_I 64)) as SUCFAIL.
-    forward SUCFAIL; [intros contra; inversion contra|].
 
-    destruct SUCFAIL as [ALLOC_SUC | ALLOC_OOM].
-    - apply ErrSID_succeeds_ErrSID_runs_to with (sid:=ms_sid m) (pr := ms_prov m) in ALLOC_SUC.
-      destruct ALLOC_SUC as ((ms' & addr) & sid'' & pr'' & RUNS).
-      unfold ErrSID_runs_to in RUNS.
-      rewrite RUNS in INTERP.
-      cbn in INTERP.
-      go_in INTERP.
-      cbn in INTERP.
-      go_in INTERP.
-      cbn in INTERP.
+    unfold interp_mcfg4 in *.
+    unfold model_undef in *.
 
-      apply interp_prop_ret_inv in INTERP.
-      destruct INTERP as ((ms'' & (lenv & ls & res)) & REF & RES).
+    destruct INTERP as [t_pre [INTERP UNDEF]].
+    unfold interp_memory_prop in INTERP.
+    unfold t_alloc in INTERP.
+    cbn in INTERP.
+    rewrite interp_intrinsics_bind in INTERP.
+    go_in INTERP.
+    rewrite bind_trigger in INTERP.
+    repeat setoid_rewrite bind_ret_l in INTERP.
+    setoid_rewrite interp_local_stack_ret in INTERP.
+    repeat setoid_rewrite bind_ret_l in INTERP.
+    
+    setoid_rewrite interp_intrinsics_ret in INTERP.
+    setoid_rewrite interp_global_ret in INTERP.
+    setoid_rewrite interp_local_stack_ret in INTERP.
 
-      inversion REF; subst.
-      inversion H4; subst.
-      inversion H6; subst.
+    rewrite interp_prop_vis in INTERP.
 
-      
-      (* Any dv that res concretizes to, UVALUE_None can also
-         concretize to...
+    (* Maybe write a lemma to unfold this... *)
+    cbn in INTERP.
+    Import MMEP.MemSpec.
+    unfold my_handle_memory_prop in INTERP.
+    Opaque bind ret.
+    Opaque MMEP.MemSpec.allocate_dtyp_spec.
+    cbn in INTERP.
+    unfold bind_PropT in INTERP.
+    destruct INTERP as [ta [k [ALLOC [K INTERP]]]].
+    destruct ALLOC as [sid' [ms' ALLOC]].
 
-         This doesn't necessarily tell me that 
-       *)
+    pose proof allocate_dtyp_spec_inv m (DTYPE_I 64) as ALLOCINV.
+    forward ALLOCINV. intros CONTRA; inv CONTRA.
 
-      exists (ret (ms'', (lenv, (ls, res)))).
-      cbn.
+    Transparent bind ret.
+    Transparent MMEP.MemSpec.allocate_dtyp_spec.
+
+    (* TODO: move this *)
+    Arguments MMEP.MemSpec.allocate_dtyp_spec dt : simpl never.
+
+    cbn in ALLOC.
+    unfold MemPropT_lift_PropT_fresh in ALLOC.
+    cbn in ALLOC.
+
+    Transparent bind ret.
+    Transparent MMEP.MemSpec.allocate_dtyp_spec.
+
+    destruct ALLOC as [ALLOC_UB | [ALLOC_ERR | [ALLOC_OOM | ALLOC_SUC]]].
+    - (* UB *)
+      destruct ALLOC_UB as [ub_msg [ALLOC_UB | [sab [a [ALLOC_UB []]]]]].
+      apply ALLOCINV in ALLOC_UB.
+      destruct ALLOC_UB as [[ms_final [ptr ALLOC_UB]] | [oom_msg ALLOC_UB]];
+        inv ALLOC_UB.
+    - (* ERR *)
+      destruct ALLOC_ERR as [err_msg [MAP [spec_msg [ALLOC_ERR | [sab [a [ALLOC_ERR []]]]]]]].
+      apply ALLOCINV in ALLOC_ERR.
+      destruct ALLOC_ERR as [[ms_final [ptr ALLOC_ERR]] | [oom_msg ALLOC_ERR]];
+        inv ALLOC_ERR.
+    - (* OOM *)
+      destruct ALLOC_OOM as [err_msg [MAP [spec_msg [ALLOC_OOM | [sab [a [ALLOC_OOM []]]]]]]].
+      apply ALLOCINV in ALLOC_OOM.
+      destruct ALLOC_OOM as [[ms_final [ptr ALLOC_OOM]] | [oom_msg ALLOC_OOM]];
+        inv ALLOC_OOM.
+
+      Import Raise.
+      apply raiseOOM_map_itree_inv in MAP.
+      rewrite MAP in K.
+      rewrite (@rbm_raise_bind _ _ _ _ _ (RaiseBindM_OOM _)) in K.
+      apply raiseOOM_map_itree_inv in K.
+
+      (* TODO: why can't I just do this rewrite? *)
+      rewrite K in UNDEF.
+
+      (* TODO: should be clear that t' is raiseOOM as well *)
+      (* Should be able to have a lemma for that *)
+      assert (t' ≈ raiseOOM err_msg) as T' by admit.
+
+      exists (Ret5 genv (lenv, stack) sid m (DVALUE_I1 DynamicValues.Int1.one)).
       split.
+      +  exists (Ret5 genv (lenv, stack) sid m (DVALUE_I1 DynamicValues.Int1.one)).
+         (* exists (Ret2 genv (lenv, stack) (DVALUE_I1 DynamicValues.Int1.one)). *)
+         split.
+         * cbn.
+           go_prime.
 
-      { unfold interp_mcfg4.
-        go.
-
-        (* TODO: lemma about model_undef? *)
-        unfold model_undef.
-        apply interp_prop_ret_refine.
-        repeat split; eauto.
-      }
-
-      right.
-      
-      apply OOM.eutt_refine_oom_h.
-      typeclasses eauto.
-      typeclasses eauto.
-
-      rewrite RES.
-      reflexivity.
-    - unfold ErrSID_OOMs in ALLOC_OOM.
-      specialize (ALLOC_OOM (ms_sid m) (ms_prov m)).
-      break_match_hyp; inversion ALLOC_OOM.
-
-      destruct (runErrSID (allocate (ms_memory_stack m) (DTYPE_I 64)) (ms_sid m) (ms_prov m)) eqn:Halloc.
-      destruct p.
-      assert (s0 = inl o). admit.
-      subst.
-      destruct o.
-      cbn in *.
-      go_in INTERP.
-
-      setoid_rewrite Raise.raiseOOM_bind_itree in INTERP.
-
-      eexists.
-
+           (* TODO: ret lemma for interp_memory_prop *)
+           unfold interp_memory_prop.
+           cbn.
+           rewrite map_ret.
+           eapply interp_prop_ret_refine; reflexivity.
+         * red.
+           eapply interp_prop_ret_pure; eauto.
+      + rewrite T'.
+        eapply refine_oom_h_raise_oom; typeclasses eauto.
+    - (* Success *)
+      exists (Ret5 genv (lenv, stack) sid m (DVALUE_I1 DynamicValues.Int1.one)).
       split.
+      +  exists (Ret5 genv (lenv, stack) sid m (DVALUE_I1 DynamicValues.Int1.one)).
+         (* exists (Ret2 genv (lenv, stack) (DVALUE_I1 DynamicValues.Int1.one)). *)
+         split.
+         * cbn.
+           go_prime.
 
-      { unfold interp_mcfg4.
-        go.
+           (* TODO: ret lemma for interp_memory_prop *)
+           unfold interp_memory_prop.
+           cbn.
+           rewrite map_ret.
+           eapply interp_prop_ret_refine; reflexivity.
+         * red.
+           eapply interp_prop_ret_pure; eauto.
+      + (* t' is the successful result of t_alloc *)
+        destruct ALLOC_SUC as [sid'' [ ms'' [x [MAP ALLOC_SUC]]]].        
+        destruct ALLOC_SUC as [ms''' [a [ALLOC [MEQ XEQ]]]].
+        subst.
 
-        unfold model_undef.
-        apply interp_prop_ret_pure.
-        typeclasses eauto.
-      }
+        apply itree_map_ret_inv in MAP as [x [TA EQ]].
+        rewrite TA in K.
+        setoid_rewrite bind_ret_l in K.
 
-      right.
-
-      (* TODO: Lemma to get this information from INTERP *)
-      assert (t' = LLVMEvents.raiseOOM s0).
-      admit.
-
-      rewrite H.
-
-      (* TODO: Lemma about refine_OOM_h and raiseOOM *)
-      cbn.
-      unfold OOM.refine_OOM_h.
-
-      cbn.
-      constructor.
-    - cbn.
-      unfold interp_mcfg4.
-      unfold model_undef.
-      go.
-
-      epose proof interp_prop_refl.
-      unfold Proper, respectful in *.
-
-      eapply interp_prop_ret_pure; typeclasses eauto.
-    - right.
-      Import OOM.
-
-      unfold refine_OOM_h.
-
-      Require Import Stack.
-      Require Import Global.
-      cbn.
-      
-      (* I basically need to show that t' is the same as t_alloc, but
-         with a different effects signature..
-
-         I.e., it either OOMs or it returns UVALUE_None
-       *)
-      pose proof (@allocate_succeeds_or_OOMs (ms_memory_stack m) (DTYPE_I 64)) as SUCFAIL.
-      forward SUCFAIL; [intros contra; inversion contra|].
-
-      destruct SUCFAIL as [ALLOC_SUC | ALLOC_OOM].
-
-      + apply ErrSID_succeeds_ErrSID_runs_to with (sid:=ms_sid m) (pr := ms_prov m) in ALLOC_SUC.
-        destruct ALLOC_SUC as ((ms' & addr) & sid'' & pr'' & RUNS).
-        unfold ErrSID_runs_to in RUNS.
-        rewrite RUNS in INTERP.
-        cbn in INTERP.
-        go_in INTERP.
-        cbn in INTERP.
-        go_in INTERP.
-        cbn in INTERP.
+        specialize (INTERP x).
+        forward INTERP.
+        { constructor; auto.
+        }
 
         apply interp_prop_ret_inv in INTERP.
-        destruct INTERP as (r2 & _ & RES).
-        rewrite RES.
+        destruct INTERP as [[lenv' [stack' res']] [R2 K']].
+        rewrite K' in K.
 
+        apply itree_map_ret_inv in K.
+        destruct K as [[ms'''' [sid'''' [lenv'''' [stack'''' res]]]] [TPRE ENV]].
+        inv ENV.
+
+        unfold model_undef_h in UNDEF.
+
+        (* TODO: why can't I just do this rewrite? *)
+        rewrite TPRE in UNDEF.
+
+        eapply interp_prop_ret_inv in UNDEF.
+        destruct UNDEF as [r2 [RPICK T']].
+        destruct r2 as [ms''''' [sid''''' z]].
+        rewrite T'.
         cbn.
 
-        (* Won't work... *)
-        (* Just need to lift some of this proof and go back and change the existential, I think *)
-        
-        rewrite bind_ret_l in INTERP.
-        rewrite H
-          unfold ErrSID_succeeds in ALLOC_SUC.
+        inv RPICK.
+        inv R2.
 
-      + rewrite interp_intrinsics_trigger in INTERP.
-
-
-      go_in INTERP.
-
-      epose proof interp_prop_Proper_eq.
-
-      eapply interp_prop_Proper_eq in INTERP; try typeclasses eauto.
-      2 : {
-        go.
-        rewrite interp_memory_trigger.
-        cbn.
-        go.
-        cbn.
-      }
-
-      setoid_rewrite interp_intrinsics_trigger in INTERP.
-
-
-      rewrite interp_prop _bind in INTERP.
-
-
-      
-      cbn in GOAL.
-      
-      setoid_rewrite bind_trigger in INTERP.
-      unfolf
-      apply OOM.eutt_refine_oom_h; try typeclasses eauto.
-      reflexivity.
-  Qed.
+        (* Not quite reflexivity... *)
+        unfold refine_OOM_h.
+        apply interp_prop_ret_refine.
+        do 2 red.
+        unfold refine_res2, refine_res1.
+        repeat constructor; auto.
+  Admitted.
 End Finite.
